@prefix owl: <http://www.w3.org/2002/07/owl#> .
@prefix chem: <http://sweetontology.net/matr/> .
@prefix elem: <http://sweetontology.net/matrElement/> .
@prefix rela: <http://sweetontology.net/rela/> .
@prefix comp: <http://sweetontology.net/matrCompound/> .
@prefix prela: <http://sweetontology.net/relaPhysical/> .
@prefix crela: <http://sweetontology.net/relaChemical/> .
@prefix state: <http://sweetontology.net/state/> .
@prefix pstate: <http://sweetontology.net/statePhysical/> .
@prefix ion: <http://sweetontology.net/matrIon/> .
@prefix allo: <http://sweetontology.net/matrElementalMolecule/> .
@prefix rdf: <http://www.w3.org/1999/02/22-rdf-syntax-ns#> .
@prefix rdfs: <http://www.w3.org/2000/01/rdf-schema#> .
@prefix xsd: <http://www.w3.org/2001/XMLSchema#> .

<http://sweetontology.net/matrIon> a owl:Ontology ;
	owl:versionInfo "3.0.0" ;
	rdfs:label "SWEET Ontology" ;
	owl:imports <http://sweetontology.net/matrCompound> , <http://sweetontology.net/relaPhysical> , <http://sweetontology.net/matrElement> , <http://sweetontology.net/relaChemical> , <http://sweetontology.net/matrElementalMolecule> , <http://sweetontology.net/statePhysical> , <http://sweetontology.net/state> , <http://sweetontology.net/matr> , <http://sweetontology.net/rela> .

ion:Anion a owl:Class ;
	rdfs:subClassOf ion:Ion ;
	rdfs:comment "An anion is an ion that has more electrons than protons such that the atom or molecule is negatively charged. [Wikipedia]"@en .

ion:Cation a owl:Class ;
	rdfs:subClassOf ion:Ion ;
	rdfs:comment "An cation is an ion that has more protons than electrons such that the atom or molecule is positively charged. [Wikipedia]"@en .

ion:HeavyIon a owl:Class ;
	rdfs:subClassOf ion:Ion .

ion:Ion a owl:Class ;
	rdfs:subClassOf chem:Substance , _:node1boamdvpax1 .

_:node1boamdvpax1 a owl:Restriction ;
	owl:onProperty rela:hasState ;
	owl:hasValue pstate:Ionized .

ion:Ion rdfs:comment "An ion is an atom or molecule where the total number of electrons is not equal to the total number of protons, giving it a net positive or negative electrical charge. [Wikipedia]"@en .

ion:SaltIon a owl:Class ;
	rdfs:subClassOf ion:Ion .

ion:HCO3minus a ion:Ion , comp:InorganicCompound ;
	crela:hasChemical_1 elem:H ;
	crela:hasChemical_2 elem:C ;
	crela:hasChemical_3 ion:O3minus ;
	owl:sameAs ion:Bicarbonite , ion:HydrogenCarbonate .

ion:Bicarbonite a ion:Ion .

ion:HydrogenCarbonate a ion:Ion .

ion:CO3minusminus a ion:Ion , comp:InorganicCompound ;
	crela:hasChemical_1 elem:C ;
	crela:hasChemical_2 ion:O3minusminus ;
	owl:sameAs ion:Carbonate .

ion:Carbonate a ion:Ion .

ion:NO2minus a ion:Ion , comp:InorganicCompound ;
	crela:hasChemical_1 elem:N ;
	crela:hasChemical_2 ion:O2minus ;
	owl:sameAs ion:Nitrite .

ion:Nitrite a ion:Ion .

ion:NO3minus a ion:Ion , comp:InorganicCompound ;
	crela:hasChemical_1 elem:N ;
	crela:hasChemical_2 ion:O3minus ;
	owl:sameAs ion:Nitrate .

ion:Nitrate a ion:Ion .

ion:NH4plus a ion:Ion , comp:InorganicCompound ;
	crela:hasChemical_1 elem:N ;
	crela:hasChemical_2 ion:H4plus ;
	owl:sameAs ion:Ammonium .

ion:Ammonium a ion:Ion .

ion:Hplus a ion:Ion ;
	crela:hasChemical elem:H ;
	prela:hasCharge "1"^^xsd:integer .

ion:H4plus a ion:Ion ;
	crela:hasChemical allo:H4 ;
	prela:hasCharge "1"^^xsd:integer .

ion:Ominus a ion:Ion ;
	crela:hasChemical elem:O ;
	prela:hasCharge "-1"^^xsd:integer .

ion:O2minus a ion:Ion ;
	crela:hasChemical allo:O2 ;
	prela:hasCharge "-1"^^xsd:integer .

ion:O3minus a ion:Ion ;
	crela:hasChemical allo:O3 ;
	prela:hasCharge "-1"^^xsd:integer .

ion:Oplus a ion:Ion ;
	crela:hasChemical elem:O ;
	prela:hasCharge "1"^^xsd:integer .

ion:O3minusminus a ion:Ion ;
	crela:hasChemical allo:O3 ;
	prela:hasCharge "-2"^^xsd:integer .
