@prefix atmp: <http://sweetontology.net/phenAtmo> .
@prefix mod: <http://sweetontology.net/reprSciModel> .
@prefix sys: <http://sweetontology.net/phenSystemComplexity> .
@prefix atmo: <http://sweetontology.net/realmAtmo> .
@prefix boun: <http://sweetontology.net/realmAtmoBoundaryLayer> .
@prefix plan: <http://sweetontology.net/realm> .
@prefix fog: <http://sweetontology.net/phenAtmoFog> .
@prefix phen: <http://sweetontology.net/phen> .
@prefix water: <http://sweetontology.net/matrWater> .
@prefix orog: <http://sweetontology.net/realmLandOrographic> .
@prefix chem: <http://sweetontology.net/matr> .
@prefix trela: <http://sweetontology.net/relaTime> .
@prefix srela: <http://sweetontology.net/relaSpace> .
@prefix rela: <http://sweetontology.net/rela> .
@prefix day: <http://sweetontology.net/reprTimeDay> .
@prefix wave: <http://sweetontology.net/phenWave> .
@prefix inst: <http://sweetontology.net/phenFluidInstability> .
@prefix wind: <http://sweetontology.net/phenAtmoWind> .
@prefix scale: <http://sweetontology.net/stateSpaceScale> .
@prefix owl: <http://www.w3.org/2002/07/owl#> .
@prefix rdf: <http://www.w3.org/1999/02/22-rdf-syntax-ns#> .
@prefix rdfs: <http://www.w3.org/2000/01/rdf-schema#> .
@prefix xsd: <http://www.w3.org/2001/XMLSchema#> .

<http://sweetontology.net/phenAtmo> a owl:Ontology ;
	owl:versionInfo "3.0.0" ;
	rdfs:label "SWEET Ontology" ;
	owl:imports <http://sweetontology.net/realmAtmo> , <http://sweetontology.net/realmAtmoBoundaryLayer> , <http://sweetontology.net/phenFluidInstability> , <http://sweetontology.net/relaTime> , <http://sweetontology.net/relaSpace> , <http://sweetontology.net/rela> , <http://sweetontology.net/reprTimeDay> , <http://sweetontology.net/matr> , <http://sweetontology.net/realmLandOrographic> , <http://sweetontology.net/phenAtmoFog> , <http://sweetontology.net/realm> , <http://sweetontology.net/phen> , <http://sweetontology.net/matrWater> , <http://sweetontology.net/phenWave> , <http://sweetontology.net/phenAtmoWind> , <http://sweetontology.net/stateSpaceScale> , <http://sweetontology.net/reprSciModel> , <http://sweetontology.net/phenSystemComplexity> .

<http://sweetontology.net/phenAtmo/MeteorologicalPhenomena> a owl:Class ;
	rdfs:subClassOf <http://sweetontology.net/phenAtmo/AtmosphericPhenomena> .

<http://sweetontology.net/phenAtmo/AtmosphericPhenomena> a owl:Class ;
	rdfs:subClassOf <http://sweetontology.net/phen/PlanetaryPhenomena> .

<http://sweetontology.net/phenAtmo/AirMass> a owl:Class ;
	rdfs:subClassOf <http://sweetontology.net/matr/Air> , <http://sweetontology.net/reprSciModel/Model> ;
	rdfs:label "Air Mass" ;
	rdfs:comment "A widespread body of air, the properties of which can be identified as 1) having been established while that air was situated over a particular region of the earth's surface (airmass source region), and 2) undergoing specific modifications while in transit away from the source region." .

<http://sweetontology.net/phenAtmo/Weather> a owl:Class ;
	rdfs:subClassOf <http://sweetontology.net/phenAtmo/MeteorologicalPhenomena> ;
	owl:equivalentClass <http://sweetontology.net/phenAtmo/WeatherCondition> .

<http://sweetontology.net/phenAtmo/WeatherCondition> a owl:Class .

<http://sweetontology.net/phenAtmo/Thermal> a owl:Class ;
	rdfs:subClassOf <http://sweetontology.net/phenAtmo/MeteorologicalPhenomena> .

<http://sweetontology.net/phenAtmo/OrographicLifting> a owl:Class ;
	rdfs:subClassOf <http://sweetontology.net/phenFluidInstability/Lifting> , _:node1boame1m7x1 .

_:node1boame1m7x1 a owl:Restriction ;
	owl:onProperty <http://sweetontology.net/rela/hasPhenomena> ;
	owl:someValuesFrom <http://sweetontology.net/realmLandOrographic/Orographic> .

<http://sweetontology.net/phenAtmo/OrographicLifting> rdfs:comment "Ascending air flow caused by mountains.  Mechanisms that produce the lifting fall into two broad categories: 1) the upward deflection of horizontal larger-scale flow by the orography acting as an obstacle or barrier; or 2) the daytime heating of mountain surfaces to produce anabatic flow along the slopes and updrafts in the vicinity of the peaks."@en .

<http://sweetontology.net/phenAtmo/NocturnalCooling> a owl:Class ;
	rdfs:subClassOf <http://sweetontology.net/phen/RadiationalCooling> , _:node1boame1m7x2 .

_:node1boame1m7x2 a owl:Restriction ;
	owl:onProperty <http://sweetontology.net/relaTime/hasTime> ;
	owl:allValuesFrom <http://sweetontology.net/reprTimeDay/Nocturnal> .

<http://sweetontology.net/phenAtmo/NocturnalCooling> rdfs:comment "The lowering of temperature during night time, due to a net loss of radiant energy."@en .

<http://sweetontology.net/phenAtmo/MixedLayerCappingInversion> a owl:Class ;
	rdfs:subClassOf <http://sweetontology.net/phenAtmo/CappingInversion> ;
	rdfs:comment "The statically stable layer of air at the top of the atmospheric boundary layer. Because the troposphere is statically stable on the average (i.e., potential temperature increases with height), and because turbulence in the boundary layer causes potential temperatures to become somewhat well mixed there, conservation of heat requires that there be a potential temperature increase (i.e., a temperature step or inversion) at the top of the boundary layer. It is this inversion that separates the boundary layer from the rest of the troposphere by limiting the domain of turbulence. It is also responsible for trapping pollutants near the ground during fair weather."@en .

<http://sweetontology.net/phenAtmo/CappingInversion> a owl:Class ;
	rdfs:subClassOf <http://sweetontology.net/phenAtmo/MeteorologicalPhenomena> ;
	rdfs:comment "A statically stable layer at the top of the atmospheric boundary layer."@en .

<http://sweetontology.net/phenAtmo/GroundInversion> a owl:Class ;
	rdfs:subClassOf <http://sweetontology.net/phenAtmo/MeteorologicalPhenomena> ;
	rdfs:comment "An air layer with its base at the ground surface and in which temperature increases with height. These often form at night over land under clear skies and are statically stable. See inversion, lapse rate."@en .

<http://sweetontology.net/phenAtmo/MoisturePooling> a owl:Class ;
	rdfs:subClassOf <http://sweetontology.net/phenAtmo/MeteorologicalPhenomena> ;
	rdfs:comment "The development of an area in the boundary layer (e.g., often observed on surface or 850-mb charts) where moisture values become higher than in the surrounding region. Moisture pooling typically occurs in an area of low-level convergence during the warm (growing) season, and can have a significant effect on convection initiation and evolution."@en .

<http://sweetontology.net/phenAtmo/MixedLayerEvolution> a owl:Class ;
	rdfs:subClassOf <http://sweetontology.net/phenSystemComplexity/Evolution> , _:node1boame1m7x3 .

_:node1boame1m7x3 a owl:Restriction ;
	owl:onProperty <http://sweetontology.net/rela/hasRealm> ;
	owl:allValuesFrom <http://sweetontology.net/realmAtmoBoundaryLayer/MixedLayer> .

<http://sweetontology.net/phenAtmo/MixedLayerEvolution> rdfs:comment "The three-part change of the atmospheric boundary layer that typically occurs during fair weather over land on sunny days. In the early morning, the mixed layer is shallow, slowly deepening, cool (in a potential temperature sense), and is capped by the remains of the stable boundary layer from the previous night. In mid- to late morning, the top of the mixed layer exhibits rapid rise as heating eliminates the nocturnal inversion, and the mixed layer grows through the residual layer. The third stage in late morning and afternoon is that of a deep (order of 1?2 km) convective boundary layer of relatively constant depth."@en .

<http://sweetontology.net/phenAtmo/AtmosphericDisturbance> a owl:Class ;
	rdfs:subClassOf <http://sweetontology.net/phenAtmo/AtmosphericWave> .

<http://sweetontology.net/phenAtmo/MesoscaleDisturbance> a owl:Class ;
	rdfs:subClassOf <http://sweetontology.net/phenAtmo/AtmosphericDisturbance> , _:node1boame1m7x4 .

_:node1boame1m7x4 a owl:Restriction ;
	owl:onProperty <http://sweetontology.net/relaSpace/hasSpatialScale> ;
	owl:hasValue <http://sweetontology.net/stateSpaceScale/Mesoscale> .

<http://sweetontology.net/phenAtmo/MesoscaleDisturbance> rdfs:comment "A disturbance where the atmospheric feature has a Rossby number of order 1 and exhibits a horizontal scale comparable to the Rossby radius of deformation. For such systems, both ageostrophic advection and rotational influences are important."@en .

<http://sweetontology.net/phenAtmo/AtmosphericWave> a owl:Class ;
	rdfs:subClassOf <http://sweetontology.net/phenWave/FluidWave> , _:node1boame1m7x5 .

_:node1boame1m7x5 a owl:Restriction ;
	owl:onProperty <http://sweetontology.net/rela/hasRealm> ;
	owl:allValuesFrom <http://sweetontology.net/realm/Atmosphere> .

<http://sweetontology.net/phenAtmo/FrontalWave> a owl:Class ;
	rdfs:subClassOf <http://sweetontology.net/phenAtmo/AtmosphericWave> ;
	rdfs:comment "A horizontal wavelike deformation of a front in the lower levels, commonly associated with a maximum of cyclonic circulation in the adjacent flow. It may develop into a wave cyclone."@en .

<http://sweetontology.net/phenAtmo/EasterlyWave> a owl:Class ;
	rdfs:subClassOf <http://sweetontology.net/phenAtmo/AtmosphericWave> , _:node1boame1m7x6 .

_:node1boame1m7x6 a owl:Restriction ;
	owl:onProperty <http://sweetontology.net/rela/hasPhenomena> ;
	owl:allValuesFrom <http://sweetontology.net/phenAtmoWind/EasterlyWind> .

<http://sweetontology.net/phenAtmo/EasterlyWave> rdfs:comment "A migratory wavelike disturbance of the tropical easterlies."@en .

<http://sweetontology.net/phenAtmo/MountainWave> a owl:Class ;
	rdfs:subClassOf <http://sweetontology.net/phenAtmo/AtmosphericWave> , _:node1boame1m7x7 .

_:node1boame1m7x7 a owl:Restriction ;
	owl:onProperty <http://sweetontology.net/rela/hasRealm> ;
	owl:allValuesFrom <http://sweetontology.net/realmLandOrographic/Mountain> .

<http://sweetontology.net/phenAtmo/MountainWave> rdfs:comment "An atmospheric gravity wave, formed when stable air flow passes over a mountain or mountain barrier."@en .

<http://sweetontology.net/phenAtmo/FoehnWave> a owl:Class ;
	rdfs:subClassOf <http://sweetontology.net/phenAtmo/MountainWave> ;
	rdfs:comment "Mountain waves, lee waves, or trapped lee waves in the air stream flowing over the mountain barrier that occur in association with foehn conditions. The Moazagotl is one example of a foehn wave made visible by lee-wave clouds."@en .

<http://sweetontology.net/phenAtmo/LeeWave> a owl:Class ;
	rdfs:subClassOf <http://sweetontology.net/phenAtmo/MountainWave> ;
	rdfs:comment "1. Any wave disturbance that is caused by, and is therefore stationary with respect to, some barrier in the fluid flow. Whether the wave is a gravity wave, inertia wave, barotropic wave, etc., will depend on the structure of the fluid and the dimensions of the barrier. 2. A mountain wave occurring to the lee of a mountain or mountain barrier. These waves can become visible in the form of lenticular or trapped lee-wave clouds."@en .

<http://sweetontology.net/phenAtmo/Icing> a owl:Class ;
	rdfs:subClassOf <http://sweetontology.net/phenAtmo/MeteorologicalPhenomena> .

<http://sweetontology.net/phenAtmo/KillingFreeze> a owl:Class ;
	rdfs:subClassOf <http://sweetontology.net/matrWater/Frost> ;
	rdfs:comment "The occurrence of air temperature below 0 C (32F) that kills annual vegetation without formation of frost crystals on surfaces. See freeze, dry freeze, hard freeze, light freeze."@en .

<http://sweetontology.net/phenAtmo/LightFreeze> a owl:Class ;
	rdfs:subClassOf <http://sweetontology.net/matrWater/Frost> ;
	rdfs:comment "The occurrence of air temperature below 0 C (32F) that kills some, but not all, annual vegetation. This often occurs in the 0 to -1 C (32 30 F) range."@en .

<http://sweetontology.net/phenAtmo/LightFrost> a owl:Class ;
	rdfs:subClassOf <http://sweetontology.net/matrWater/Frost> ;
	rdfs:comment "A thin and more or less patchy deposit of hoarfrost on surface objects and vegetation."@en .

<http://sweetontology.net/phenAtmo/Sunlit> a owl:Class ;
	rdfs:subClassOf <http://sweetontology.net/phenAtmo/WeatherCondition> .

<http://sweetontology.net/phenAtmo/Obscuration> a owl:Class ;
	rdfs:subClassOf <http://sweetontology.net/phenAtmoFog/Fog> .

<http://sweetontology.net/phenAtmo/Whiteout> a owl:Class ;
	rdfs:subClassOf <http://sweetontology.net/phenAtmo/Obscuration> ;
	rdfs:comment "An atmospheric optical phenomenon in which the observer appears to be engulfed in a uniformly white glow."@en .

<http://sweetontology.net/phenAtmo/Rainbow> a owl:Class ;
	rdfs:subClassOf <http://sweetontology.net/phenAtmo/MeteorologicalPhenomena> .

<http://sweetontology.net/phenAtmo/Sunlight> a owl:Class ;
	rdfs:subClassOf <http://sweetontology.net/phen/RadiativeHeating> ;
	rdfs:comment "Sunlight, in the broad sense, is the total spectrum of the electromagnetic radiation given off by the Sun. On Earth, sunlight is filtered through the atmosphere, and the solar radiation is obvious as daylight when the Sun is above the horizon. This is usually during the hours known as day. Near the poles in summer, sunlight also occurs during the hours known as night and in the winter at the poles sunlight may not occur at any time. When the direct radiation is not blocked by clouds, it is experienced as sunshine, a combination of bright light and heat. Radiant heat directly produced by the radiation of the sun is different from the increase in atmospheric temperature due to the radiative heating of the atmosphere by the sun's radiation."@en .
