@prefix elec: <http://sweetontology.net/propCharge> .
@prefix light: <http://sweetontology.net/phenAtmoLightning> .
@prefix atmo: <http://sweetontology.net/phenAtmo> .
@prefix rela: <http://sweetontology.net/rela> .
@prefix precip: <http://sweetontology.net/phenAtmoPrecipitation> .
@prefix wave: <http://sweetontology.net/phenWave> .
@prefix owl: <http://www.w3.org/2002/07/owl#> .
@prefix rdf: <http://www.w3.org/1999/02/22-rdf-syntax-ns#> .
@prefix rdfs: <http://www.w3.org/2000/01/rdf-schema#> .
@prefix xsd: <http://www.w3.org/2001/XMLSchema#> .

<http://sweetontology.net/phenAtmoLightning> a owl:Ontology ;
	owl:versionInfo "3.0.0" ;
	rdfs:label "SWEET Ontology" ;
	owl:imports <http://sweetontology.net/phenAtmo> , <http://sweetontology.net/propCharge> , <http://sweetontology.net/rela> , <http://sweetontology.net/phenAtmoPrecipitation> , <http://sweetontology.net/phenWave> .

<http://sweetontology.net/phenAtmoLightning/BallLightning> a owl:Class ;
	rdfs:subClassOf <http://sweetontology.net/phenAtmoLightning/Lightning> ;
	rdfs:comment "A rare and randomly occurring bright ball of light observed floating or moving through the atmosphere close to the ground."@en .

<http://sweetontology.net/phenAtmoLightning/BeadedLightning> a owl:Class ;
	rdfs:subClassOf <http://sweetontology.net/phenAtmoLightning/Lightning> ;
	rdfs:comment "A particular aspect of a normal lightning flash occasionally seen when the observer happens to view end-on a number of segments of the irregular channel (zigzag lightning) and hence receives an impression of higher luminosity at a series of locations along the channel."@en .

<http://sweetontology.net/phenAtmoLightning/BlueJet> a owl:Class ;
	rdfs:subClassOf <http://sweetontology.net/phenAtmoLightning/Lightning> ;
	rdfs:comment "Weakly luminous upward propagating discharges, blue in color, emanating from the tops of thunderstorms."@en .

<http://sweetontology.net/phenAtmoLightning/JunctionStreamer> a owl:Class ;
	rdfs:subClassOf _:node1boame298x1 .

_:node1boame298x1 a owl:Restriction ;
	owl:onProperty <http://sweetontology.net/rela/hasPhenomena> ;
	owl:allValuesFrom <http://sweetontology.net/phenAtmoPrecipitation/Thunderstorm> .

<http://sweetontology.net/phenAtmoLightning/JunctionStreamer> rdfs:subClassOf _:node1boame298x2 .

_:node1boame298x2 a owl:Restriction ;
	owl:onProperty <http://sweetontology.net/rela/hasPhenomena> ;
	owl:allValuesFrom <http://sweetontology.net/phenAtmoLightning/Lightning> .

<http://sweetontology.net/phenAtmoLightning/JunctionStreamer> rdfs:subClassOf <http://sweetontology.net/phenAtmoLightning/Lightning> ;
	rdfs:comment "The process by which negative charge centers at successively more distant locations in a thundercloud are tapped for discharge by successive strokes of cloud-to-ground lightning."@en .

<http://sweetontology.net/phenAtmoLightning/Lightning> a owl:Class ;
	rdfs:subClassOf <http://sweetontology.net/phenAtmo/MeteorologicalPhenomena> , _:node1boame298x3 .

_:node1boame298x3 a owl:Restriction ;
	owl:onProperty <http://sweetontology.net/rela/hasPhenomena> ;
	owl:someValuesFrom <http://sweetontology.net/propCharge/ElectricPotential> .

<http://sweetontology.net/phenAtmoLightning/Lightning> rdfs:subClassOf _:node1boame298x4 .

_:node1boame298x4 a owl:Restriction ;
	owl:onProperty <http://sweetontology.net/rela/hasPhenomena> ;
	owl:allValuesFrom <http://sweetontology.net/phenAtmoLightning/Thunder> .

<http://sweetontology.net/phenAtmoLightning/Lightning> rdfs:comment "Lightning is a transient, high-current electric discharge with pathlengths measured in kilometers. The most common source of lightning is the electric charge separated in ordinary thunderstorm clouds."@en .

<http://sweetontology.net/phenAtmoLightning/ReturnStroke> a owl:Class ;
	rdfs:subClassOf <http://sweetontology.net/phenAtmoLightning/Lightning> ;
	rdfs:comment "The intense luminosity that propagates upward from earth to cloud base in the last phase of each lightning stroke of a cloud-to-ground discharge."@en .

<http://sweetontology.net/phenAtmoLightning/Thunder> a owl:Class ;
	rdfs:subClassOf <http://sweetontology.net/phenAtmo/MeteorologicalPhenomena> , _:node1boame298x5 .

_:node1boame298x5 a owl:Restriction ;
	owl:onProperty <http://sweetontology.net/rela/hasPhenomena> ;
	owl:allValuesFrom <http://sweetontology.net/phenWave/Sound> .

<http://sweetontology.net/phenAtmoLightning/Thunder> rdfs:comment "The sound emitted by rapidly expanding gases along the channel of a lightning discharge."@en .
