@prefix fog: <http://sweetontology.net/phenAtmoFog> .
@prefix sed: <http://sweetontology.net/matrSediment> .
@prefix orog: <http://sweetontology.net/realmLandOrographic> .
@prefix comp: <http://sweetontology.net/matrCompound> .
@prefix meso: <http://sweetontology.net/phenAtmoWindMesoscale> .
@prefix srela: <http://sweetontology.net/relaSpace> .
@prefix crela: <http://sweetontology.net/relaChemical> .
@prefix prela: <http://sweetontology.net/relaPhysical> .
@prefix rela: <http://sweetontology.net/rela> .
@prefix statec: <http://sweetontology.net/procStateChange> .
@prefix coast: <http://sweetontology.net/realmLandCoastal> .
@prefix water: <http://sweetontology.net/matrWater> .
@prefix cloud: <http://sweetontology.net/phenAtmoCloud> .
@prefix mix: <http://sweetontology.net/phenMixing> .
@prefix planet: <http://sweetontology.net/realm> .
@prefix phen: <http://sweetontology.net/phen> .
@prefix precip: <http://sweetontology.net/phenAtmoPrecipitation> .
@prefix front: <http://sweetontology.net/phenAtmoFront> .
@prefix trans: <http://sweetontology.net/phenFluidTransport> .
@prefix owl: <http://www.w3.org/2002/07/owl#> .
@prefix rdf: <http://www.w3.org/1999/02/22-rdf-syntax-ns#> .
@prefix rdfs: <http://www.w3.org/2000/01/rdf-schema#> .
@prefix xsd: <http://www.w3.org/2001/XMLSchema#> .

<http://sweetontology.net/phenAtmoFog> a owl:Ontology ;
	owl:versionInfo "3.0.0" ;
	rdfs:label "SWEET Ontology" ;
	owl:imports <http://sweetontology.net/matrSediment> , <http://sweetontology.net/phenAtmoWindMesoscale> , <http://sweetontology.net/procStateChange> , <http://sweetontology.net/matrWater> , <http://sweetontology.net/phenAtmoCloud> , <http://sweetontology.net/realmLandCoastal> , <http://sweetontology.net/relaSpace> , <http://sweetontology.net/relaChemical> , <http://sweetontology.net/relaPhysical> , <http://sweetontology.net/rela> , <http://sweetontology.net/matrCompound> , <http://sweetontology.net/realm> , <http://sweetontology.net/phen> , <http://sweetontology.net/phenAtmoPrecipitation> , <http://sweetontology.net/phenMixing> , <http://sweetontology.net/phenFluidTransport> , <http://sweetontology.net/phenAtmoFront> , <http://sweetontology.net/realmLandOrographic> .

<http://sweetontology.net/phenAtmoFog/AdvectionFog> a owl:Class ;
	rdfs:subClassOf <http://sweetontology.net/phenAtmoFog/Fog> , _:node1boame1vvx1 .

_:node1boame1vvx1 a owl:Restriction ;
	owl:onProperty <http://sweetontology.net/rela/hasPhenomena> ;
	owl:allValuesFrom <http://sweetontology.net/phenFluidTransport/Advection> .

<http://sweetontology.net/phenAtmoFog/AdvectionFog> rdfs:label "AdvectionFog" ;
	rdfs:comment "A type of fog caused by the advection of moist air over a cold surface, and the consequent cooling of that air to below its dewpoint." .

<http://sweetontology.net/phenAtmoFog/EvaporationFog> a owl:Class ;
	rdfs:subClassOf <http://sweetontology.net/phenAtmoFog/Fog> , _:node1boame1vvx2 .

_:node1boame1vvx2 a owl:Restriction ;
	owl:onProperty <http://sweetontology.net/relaPhysical/hasStateChange> ;
	owl:allValuesFrom <http://sweetontology.net/procStateChange/Evaporation> .

<http://sweetontology.net/phenAtmoFog/EvaporationFog> rdfs:comment "Fog formed as a result of evaporation of water that is warmer than the air."@en .

<http://sweetontology.net/phenAtmoFog/Fog> a owl:Class ;
	rdfs:subClassOf <http://sweetontology.net/phenAtmoCloud/Stratiform> , _:node1boame1vvx3 .

_:node1boame1vvx3 a owl:Restriction ;
	owl:allValuesFrom <http://sweetontology.net/realm/PlanetarySurface> ;
	owl:onProperty <http://sweetontology.net/rela/hasRealm> .

<http://sweetontology.net/phenAtmoFog/Fog> rdfs:comment "Water droplets suspended in the atmosphere in the vicinity the earth's surface that affect visibility."@en .

<http://sweetontology.net/phenAtmoFog/FreezingFog> a owl:Class ;
	rdfs:subClassOf <http://sweetontology.net/phenAtmoFog/Fog> , _:node1boame1vvx4 .

_:node1boame1vvx4 a owl:Restriction ;
	owl:onProperty <http://sweetontology.net/relaPhysical/hasStateChange> ;
	owl:allValuesFrom <http://sweetontology.net/procStateChange/Freezing> .

<http://sweetontology.net/phenAtmoFog/FreezingFog> rdfs:comment "A fog the droplets of which freeze upon contact with exposed objects and form a coating of rime and/or glaze."@en .

<http://sweetontology.net/phenAtmoFog/FrontalFog> a owl:Class ;
	rdfs:subClassOf _:node1boame1vvx5 .

_:node1boame1vvx5 a owl:Restriction ;
	owl:onProperty <http://sweetontology.net/rela/hasPhenomena> ;
	owl:allValuesFrom <http://sweetontology.net/phenAtmoFront/Front> .

<http://sweetontology.net/phenAtmoFog/FrontalFog> rdfs:subClassOf <http://sweetontology.net/phenAtmoFog/Fog> ;
	rdfs:comment "Fog associated with frontal zones and frontal passages. It is usually divided into three types: warm-front prefrontal fog; cold-front post-frontal fog; and frontal-passage fog. The first two types are a result of rain falling into cold stable air and raising the dewpoint temperature. Frontal-passage fog can result from the ?mixing of warm and cold air masses in the frontal zone? or by ?sudden cooling of air over moist ground.?"@en .

<http://sweetontology.net/phenAtmoFog/Garua> a owl:Class ;
	rdfs:subClassOf <http://sweetontology.net/phenAtmoFog/Fog> ;
	rdfs:comment "A dense fog and/or drizzle from low stratus on the west coast of South America. It creates a raw, cold atmosphere that may last for weeks in winter and supplies a limited amount of moisture to the area."@en .

<http://sweetontology.net/phenAtmoFog/GroundFog> a owl:Class ;
	rdfs:subClassOf <http://sweetontology.net/phenAtmoFog/Fog> , _:node1boame1vvx6 .

_:node1boame1vvx6 a owl:Restriction ;
	owl:onProperty <http://sweetontology.net/relaSpace/near> ;
	owl:allValuesFrom <http://sweetontology.net/realm/PlanetarySurface> .

<http://sweetontology.net/phenAtmoFog/GroundFog> rdfs:comment "1. According to U.S. weather observing practice, a fog that hides less than 0.6 of the sky and does not extend to the base of any clouds that may lie above it. As an obstruction to vision in an aviation weather observation, ground fog is encoded GF. 2. See radiation fog."@en .

<http://sweetontology.net/phenAtmoFog/Haar> a owl:Class ;
	rdfs:subClassOf <http://sweetontology.net/phenAtmoFog/Fog> , _:node1boame1vvx7 .

_:node1boame1vvx7 a owl:Restriction ;
	owl:onProperty <http://sweetontology.net/rela/hasRealm> ;
	owl:allValuesFrom <http://sweetontology.net/realmLandCoastal/Coastal> .

<http://sweetontology.net/phenAtmoFog/Haar> rdfs:comment "A name applied to a wet sea fog or very fine drizzle that drifts in from the sea in coastal districts of eastern Scotland and northeastern England. It occurs most frequently in summer."@en .

<http://sweetontology.net/phenAtmoFog/HighFog> a owl:Class ;
	rdfs:subClassOf <http://sweetontology.net/phenAtmoFog/MountainFog> ;
	rdfs:comment "In the US, the frequent fog on the slopes of the coastal mountains of California, especially applied when the fog overtops the range and extends as stratus over the leeward valleys."@en .

<http://sweetontology.net/phenAtmoFog/IceFog> a owl:Class ;
	rdfs:subClassOf <http://sweetontology.net/phenAtmoFog/Fog> , _:node1boame1vvx8 .

_:node1boame1vvx8 a owl:Restriction ;
	owl:onProperty <http://sweetontology.net/relaChemical/hasSubstance> ;
	owl:allValuesFrom <http://sweetontology.net/matrWater/Ice> .

<http://sweetontology.net/phenAtmoFog/IceFog> rdfs:comment "A type of fog, composed of suspended particles of ice, partly ice crystals 20 to 100 m in diameter, but chiefly, especially when dense, droxtals 12?20 m in diameter. It occurs at very low temperatures, and usually in clear, calm weather in high latitudes. The sun is usually visible and may cause halo phenomena. Ice fog is rare at temperatures warmer than -30?C, and increases in frequency with decreasing temperature until it is almost always present at air temperatures of -45?C in the vicinity of a source of water vapor. Such sources are the open water of fast-flowing streams or of the sea, herds of animals, volcanoes, and especially products of combustion for heating or propulsion. At temperatures warmer than -30?C, these sources can cause steam fog of liquid water droplets, which may turn into ice fog when cooled (see frost smoke). See ice-crystal haze, arctic mist."@en .

<http://sweetontology.net/phenAtmoFog/MixingFog> a owl:Class ;
	rdfs:subClassOf <http://sweetontology.net/phenAtmoFog/Fog> , _:node1boame1vvx9 .

_:node1boame1vvx9 a owl:Restriction ;
	owl:onProperty <http://sweetontology.net/rela/hasPhenomena> ;
	owl:someValuesFrom <http://sweetontology.net/phenMixing/Mixing> .

<http://sweetontology.net/phenAtmoFog/MixingFog> rdfs:comment "Fog, light and of short duration, produced by the mixing of two moist but nonsaturated air masses with different temperatures."@en .

<http://sweetontology.net/phenAtmoFog/MonsoonFog> a owl:Class ;
	rdfs:subClassOf <http://sweetontology.net/phenAtmoFog/Fog> , _:node1boame1vvx10 .

_:node1boame1vvx10 a owl:Restriction ;
	owl:onProperty <http://sweetontology.net/rela/hasPhenomena> ;
	owl:allValuesFrom <http://sweetontology.net/phenAtmoPrecipitation/Monsoon> .

<http://sweetontology.net/phenAtmoFog/MonsoonFog> rdfs:subClassOf _:node1boame1vvx11 .

_:node1boame1vvx11 a owl:Restriction ;
	owl:onProperty <http://sweetontology.net/rela/hasPhenomena> ;
	owl:allValuesFrom <http://sweetontology.net/phenFluidTransport/Advection> .

<http://sweetontology.net/phenAtmoFog/MonsoonFog> rdfs:comment "An advection fog produced as a monsoon circulation that transports warm moist air over a colder surface."@en .

<http://sweetontology.net/phenAtmoFog/MountainFog> a owl:Class ;
	rdfs:subClassOf <http://sweetontology.net/phenAtmoFog/Fog> ;
	owl:equivalentClass <http://sweetontology.net/phenAtmoFog/OrographicFog> ;
	rdfs:subClassOf _:node1boame1vvx12 .

_:node1boame1vvx12 a owl:Restriction ;
	owl:onProperty <http://sweetontology.net/rela/hasRealm> ;
	owl:someValuesFrom <http://sweetontology.net/realmLandOrographic/Mountain> .

<http://sweetontology.net/phenAtmoFog/MountainFog> rdfs:comment "Fog formed by orographic lifting to condensation of moist air up a mountain slope."@en .

<http://sweetontology.net/phenAtmoFog/OrographicFog> a owl:Class .

<http://sweetontology.net/phenAtmoFog/RadiationFog> a owl:Class ;
	rdfs:subClassOf <http://sweetontology.net/phenAtmoFog/Fog> , _:node1boame1vvx13 .

_:node1boame1vvx13 a owl:Restriction ;
	owl:onProperty <http://sweetontology.net/rela/hasPhenomena> ;
	owl:allValuesFrom <http://sweetontology.net/phen/RadiationalCooling> .

<http://sweetontology.net/phenAtmoFog/RadiationFog> rdfs:subClassOf _:node1boame1vvx14 .

_:node1boame1vvx14 a owl:Restriction ;
	owl:onProperty <http://sweetontology.net/rela/hasRealm> ;
	owl:allValuesFrom <http://sweetontology.net/realm/Land> .

<http://sweetontology.net/phenAtmoFog/RadiationFog> rdfs:comment "A common type of fog, produced over a land area when radiational cooling reduces the air temperature to or below its dewpoint."@en .

<http://sweetontology.net/phenAtmoFog/UpslopeFog> a owl:Class ;
	rdfs:subClassOf <http://sweetontology.net/phenAtmoFog/Fog> , _:node1boame1vvx15 .

_:node1boame1vvx15 a owl:Restriction ;
	owl:onProperty <http://sweetontology.net/rela/hasPhenomena> ;
	owl:allValuesFrom <http://sweetontology.net/phenAtmoWindMesoscale/UpslopeWind> .

<http://sweetontology.net/phenAtmoFog/UpslopeFog> rdfs:comment "A type of fog formed when air flows upward over rising terrain and is, consequently, adiabatically cooled to or below its dewpoint."@en .

<http://sweetontology.net/phenAtmoFog/SaltHaze> a owl:Class ;
	rdfs:subClassOf <http://sweetontology.net/phenAtmoFog/Haze> , _:node1boame1vvx16 .

_:node1boame1vvx16 a owl:Restriction ;
	owl:onProperty <http://sweetontology.net/relaChemical/hasSubstance> ;
	owl:hasValue <http://sweetontology.net/matrCompound/Salt> .

<http://sweetontology.net/phenAtmoFog/SaltHaze> rdfs:comment "A haze created by the presence of finely divided particles of sea salt in the air, usually derived from the evaporation of sea spray."@en .

<http://sweetontology.net/phenAtmoFog/Haze> a owl:Class ;
	rdfs:subClassOf <http://sweetontology.net/phenAtmoFog/Fog> ;
	rdfs:comment "Particles suspended, reducing visibility by scattering light; often a mixture of aerosols and photochemical smog."@en .

<http://sweetontology.net/phenAtmoFog/SandHaze> a owl:Class ;
	rdfs:subClassOf <http://sweetontology.net/phenAtmoFog/Haze> , _:node1boame1vvx17 .

_:node1boame1vvx17 a owl:Restriction ;
	owl:onProperty <http://sweetontology.net/relaChemical/hasSubstance> ;
	owl:someValuesFrom <http://sweetontology.net/matrSediment/Sand> .

<http://sweetontology.net/phenAtmoFog/SandHaze> rdfs:comment "Reduced visibility in the atmospheric boundary layer caused by suspended particles of soil, mixed into the air during strong winds."@en .

<http://sweetontology.net/phenAtmoFog/Smog> a owl:Class ;
	rdfs:subClassOf <http://sweetontology.net/phenAtmoFog/Fog> ;
	rdfs:comment "A natural fog contaminated by industrial pollutants, a mixture of smoke and fog."@en .

<http://sweetontology.net/phenAtmoFog/BrownCloud> a owl:Class ;
	rdfs:subClassOf <http://sweetontology.net/phenAtmoFog/Smog> ;
	rdfs:comment "Phenomenon particularly associated with smog episodes in cities such as Denver, Colorado."@en .
