@prefix ratio: <http://sweetontology.net/propDimensionlessRatio/> .
@prefix units: <http://sweetontology.net/reprSciUnits> .
@prefix mstat: <http://sweetontology.net/reprMathStatistics> .
@prefix mrela: <http://sweetontology.net/relaMath> .
@prefix mrela2: <http://sweetontology.net/relaMath/> .
@prefix screla: <http://sweetontology.net/relaSci> .
@prefix spac: <http://sweetontology.net/propSpace> .
@prefix mass: <http://sweetontology.net/propMass> .
@prefix ener: <http://sweetontology.net/propEnergy> .
@prefix quan: <http://sweetontology.net/propQuantity> .
@prefix oper: <http://sweetontology.net/reprMathOperation> .
@prefix prop: <http://sweetontology.net/prop> .
@prefix owl: <http://www.w3.org/2002/07/owl#> .
@prefix rdf: <http://www.w3.org/1999/02/22-rdf-syntax-ns#> .
@prefix rdfs: <http://www.w3.org/2000/01/rdf-schema#> .
@prefix xsd: <http://www.w3.org/2001/XMLSchema#> .

<http://sweetontology.net/propDimensionlessRatio> a owl:Ontology ;
	owl:versionInfo "3.0.0" ;
	rdfs:label "SWEET Ontology" ;
	owl:imports <http://sweetontology.net/relaMath> , <http://sweetontology.net/reprMathStatistics> , <http://sweetontology.net/relaSci> , <http://sweetontology.net/reprMathOperation> , <http://sweetontology.net/propMass> , <http://sweetontology.net/prop> , <http://sweetontology.net/propEnergy> , <http://sweetontology.net/propSpace> , <http://sweetontology.net/propQuantity> .

ratio:DimensionlessRatio a owl:Class ;
	rdfs:subClassOf <http://sweetontology.net/reprMathOperation/Ratio> , _:node1boame9p3x1 .

_:node1boame9p3x1 a owl:Restriction ;
	owl:hasValue <http://sweetontology.net/reprSciUnits/dimensionlessUnit> ;
	owl:onProperty <http://sweetontology.net/relaSci/hasDefaultUnit> .

ratio:RossbyNumber a ratio:DimensionlessRatio , ratio:DimensionlessRatio ;
	rdfs:comment "A dimensionless number relating the ratio of inertial to Coriolis forces for a given flow of a rotating fluid."@en .

ratio:FroudeNumber a ratio:DimensionlessRatio .

ratio:BulkRichardsonNumber a ratio:DimensionlessRatio ;
	mrela2:approximates ratio:RichardsonNumber ;
	rdfs:comment "An approximation to the gradient Richardson number formed by approximating local gradients by finite difference across layers."@en .

ratio:CriticalRichardsonNumber a ratio:DimensionlessRatio ;
	mrela2:hasThreshold ratio:RichardsonNumber .

ratio:GradientRichardsonNumber a ratio:DimensionlessRatio .

ratio:ReynoldsNumber a ratio:DimensionlessRatio , <http://sweetontology.net/prop/FluidProperty> ;
	rdfs:comment "The dimensionless ratio of the inertial force (∼U2/L) to the viscous force (∼ νU/L2) in the Navier–Stokes equations, where U is a characteristic velocity, L is a characteristic length, and ν is the kinematic viscosity of the fluid; thus, Re=ULv. The Reynolds number is of great importance in the theory of hydrodynamic stability and the origin of turbulence. The inertia force generates vortex stretching and nonlinear interactions and hence creates randomness. Turbulence occurs when the inertia term dominates the viscous term, that is, when the Reynolds number is large. For many engineering flows, turbulence occurs when Re > Rec, where the critical Reynolds number is roughly Rec = 2100."@en .

ratio:RichardsonNumber a ratio:DimensionlessRatio .

ratio:SonicMachNumber a ratio:DimensionlessRatio , <http://sweetontology.net/prop/MotionProperty> .

ratio:DragCoefficient a ratio:DimensionlessRatio , <http://sweetontology.net/prop/FluidProperty> .

ratio:WaterCirculationCoefficient a ratio:DimensionlessRatio ;
	rdfs:comment "The ratio of a region's total precipitation to its external precipitation originating as evaporation from the oceans as opposed to evapotranspiration from the land."@en .

ratio:LeafAreaIndex a ratio:DimensionlessRatio .

ratio:RetardationFactor a ratio:DimensionlessRatio , <http://sweetontology.net/prop/HydrogeologicalProperty> ;
	rdfs:comment "The ratio of the average linear velocity of groundwater to the velocity of the retarded constituent at C/Co=0.5."@en .

ratio:SpecificRetention a ratio:DimensionlessRatio ;
	rdfs:comment "The ratio of the Volume of water which the porous medium, after being saturated, will retain against the pull of gravity to the volume of the porous medium."@en .

ratio:SpecificStorage a ratio:DimensionlessRatio ;
	rdfs:comment "The volume of water released from or taken into storage per unit volume of the porous medium per unit change in head."@en .

ratio:SpecificYield a ratio:DimensionlessRatio ;
	rdfs:comment "The ratio of the volume of water which the porous medium after being saturated, will yield by gravity to the volume of the porous medium."@en .

ratio:AngstromExponent a ratio:DimensionlessRatio , <http://sweetontology.net/propQuantity/RadiationMediumInteractionQuantity> .

ratio:VonKarmanConstant a ratio:DimensionlessRatio , <http://sweetontology.net/propQuantity/PhysicalConstant> .

ratio:RelativePermeability a ratio:DimensionlessRatio ;
	rdfs:comment "The ratio of the effective permeability for a given flow phase to the intrinsic permeability of the porous medium (WMO, 1974). The ratio of the effective and specific permeabilities."@en .

ratio:PecletNumber a ratio:DimensionlessRatio ;
	rdfs:comment "A relationship between the advective and diffusive components of solute transport expressed as the ratio of the product of the average interstitial velocity, times the characteristic length, divided by the coefficient of molecular diffusion; small values indicate diffusion dominance, large values indicate advection dominance." .

ratio:RouseNumber a ratio:DimensionlessRatio .

ratio:SignalToNoiseRatio a ratio:DimensionlessRatio .

ratio:BowenRatio a owl:Class ;
	rdfs:subClassOf <http://sweetontology.net/reprMathOperation/Ratio> , _:node1boame9p3x2 .

_:node1boame9p3x2 a owl:Restriction ;
	owl:allValuesFrom <http://sweetontology.net/propEnergy/SensibleHeat> ;
	owl:onProperty mrela2:hasFirstOperand .

ratio:BowenRatio rdfs:subClassOf _:node1boame9p3x3 .

_:node1boame9p3x3 a owl:Restriction ;
	owl:allValuesFrom <http://sweetontology.net/propEnergy/LatentHeat> ;
	owl:onProperty mrela2:hasSecondOperand .

ratio:DepolarizationRatio a ratio:DimensionlessRatio ;
	rdfs:comment "In Raman spectroscopy, the depolarization ratio is the intensity ratio between the perpendicular component and the parallel component of the Raman scattered light."@en .

ratio:IsotopeRatio a ratio:DimensionlessRatio .

ratio:AspectRatio a ratio:DimensionlessRatio , <http://sweetontology.net/propSpace/Shape> .

ratio:Electronegativity a ratio:DimensionlessRatio , <http://sweetontology.net/propQuantity/ElectromagneticQuantity> .

ratio:PlasmaParameter a ratio:DimensionlessRatio , <http://sweetontology.net/propQuantity/ElectromagneticQuantity> .

ratio:RefractiveIndex a ratio:DimensionlessRatio , <http://sweetontology.net/propQuantity/ElectromagneticQuantity> .

ratio:HydraulicGradient a ratio:DimensionlessRatio , <http://sweetontology.net/prop/HydrogeologicalProperty> ;
	owl:sameAs ratio:DarcySlope .

ratio:DarcySlope a ratio:DimensionlessRatio .

ratio:VoidRatio a ratio:DimensionlessRatio , <http://sweetontology.net/propMass/ConsistenceProperty> .

ratio:StatisticalScore a owl:Class ;
	rdfs:subClassOf <http://sweetontology.net/prop/StatisticalSummary> .

ratio:ChiSquareValue a owl:Class ;
	rdfs:subClassOf ratio:StatisticalScore .

ratio:ReducedChiSquareValue a owl:Class ;
	rdfs:subClassOf ratio:ChiSquareValue .

ratio:ZScore a owl:Class ;
	rdfs:subClassOf ratio:StatisticalScore , _:node1boame9p3x4 .

_:node1boame9p3x4 a owl:Restriction ;
	owl:allValuesFrom <http://sweetontology.net/reprMathStatistics/ZTest> ;
	owl:onProperty mrela2:hasTest .

ratio:tScore a owl:Class ;
	rdfs:subClassOf ratio:StatisticalScore , _:node1boame9p3x5 .

_:node1boame9p3x5 a owl:Restriction ;
	owl:allValuesFrom <http://sweetontology.net/reprMathStatistics/tTest> ;
	owl:onProperty mrela2:hasTest .
