@prefix owl: <http://www.w3.org/2002/07/owl#> .
@prefix rdf: <http://www.w3.org/1999/02/22-rdf-syntax-ns#> .
@prefix rdfs: <http://www.w3.org/2000/01/rdf-schema#> .
@prefix xsd: <http://www.w3.org/2001/XMLSchema#> .
@prefix land: <http://sweetontology.net/realmLandform> .
@prefix glac: <http://sweetontology.net/realmLandGlacial> .

<http://sweetontology.net/realmLandGlacial> a owl:Ontology ;
	owl:versionInfo "3.0.0" ;
	rdfs:label "SWEET Ontology" ;
	owl:imports <http://sweetontology.net/realmLandform> .

<http://sweetontology.net/realmLandGlacial/GlacialLandform> a owl:Class ;
	rdfs:subClassOf <http://sweetontology.net/realmLandform/Landform> .

<http://sweetontology.net/realmLandGlacial/Arete> a owl:Class ;
	rdfs:subClassOf <http://sweetontology.net/realmLandGlacial/GlacialPlain> ;
	rdfs:comment "A thin, almost knife-like, ridge of rock which is typically formed when two glaciers erode parallel U-shaped valleys."@en .

<http://sweetontology.net/realmLandGlacial/Cirque> a owl:Class ;
	rdfs:subClassOf <http://sweetontology.net/realmLandGlacial/GlacialPlain> ;
	rdfs:comment "An amphitheatre-like valley head, formed at the head of a valley glacier by erosion."@en .

<http://sweetontology.net/realmLandGlacial/Esker> a owl:Class ;
	rdfs:subClassOf <http://sweetontology.net/realmLandGlacial/GlacialLandform> ;
	rdfs:comment "A long winding ridge of stratified sand and gravel, examples of which occur in glaciated and formerly glaciated regions."@en .

<http://sweetontology.net/realmLandGlacial/GlacialPlain> a owl:Class ;
	rdfs:subClassOf <http://sweetontology.net/realmLandform/Plain> , <http://sweetontology.net/realmLandGlacial/GlacialLandform> .

<http://sweetontology.net/realmLandGlacial/GlacialOutwashPlain> a owl:Class ;
	rdfs:subClassOf <http://sweetontology.net/realmLandGlacial/GlacialPlain> .

<http://sweetontology.net/realmLandGlacial/Kame> a owl:Class ;
	rdfs:subClassOf <http://sweetontology.net/realmLandGlacial/GlacialLandform> ;
	rdfs:comment "An irregularly shaped hill or mound composed of sand, gravel and till that accumulates in a depresson on a retreating glacier, and is then deposited with further melting.[Wikipedia]"@en .

<http://sweetontology.net/realmLandGlacial/Moraine> a owl:Class ;
	rdfs:subClassOf <http://sweetontology.net/realmLandGlacial/GlacialPlain> ;
	owl:equivalentClass <http://sweetontology.net/realmLandGlacial/GlacialMoraine> ;
	rdfs:comment "Any glacially formed accumulation of unconsolidated glacial debris (soil and rock) which can occur in currently glaciated and formerly glaciated regions."@en .

<http://sweetontology.net/realmLandGlacial/GlacialMoraine> a owl:Class .

<http://sweetontology.net/realmLandGlacial/OutwashFan> a owl:Class ;
	rdfs:subClassOf <http://sweetontology.net/realmLandGlacial/GlacialLandform> ;
	rdfs:comment "A fan-shaped body of sediments deposited by braided streams from a melting glacier. Sediment locked within the ice of the glacier gets transported by the streams of meltwater and deposits on the outwash plain at the terminus of the glacier."@en .

<http://sweetontology.net/realmLandGlacial/RockGlacier> a owl:Class ;
	rdfs:subClassOf <http://sweetontology.net/realmLandGlacial/GlacialLandform> ;
	rdfs:comment "Rock glaciers are distinctive geomorphological landforms of blocky detritus which may extend outward and downslope from talus cones or from glaciers or the terminal moraines of glaciers. [Wikipedia]"@en .

<http://sweetontology.net/realmLandGlacial/Sandur> a owl:Class ;
	rdfs:subClassOf <http://sweetontology.net/realmLandGlacial/GlacialOutwashPlain> ;
	rdfs:comment "A glacial outwash plain formed of sediments deposited by meltwater at the terminus of a glacier."@en .

<http://sweetontology.net/realmLandGlacial/TillPlain> a owl:Class ;
	rdfs:subClassOf <http://sweetontology.net/realmLandGlacial/GlacialPlain> ;
	owl:equivalentClass <http://sweetontology.net/realmLandGlacial/Till> ;
	rdfs:comment "An extensive flat plain of glacial till that forms when a sheet of ice becomes detached from the main body of a glacier and melts in place depositing the sediments it carried."@en .

<http://sweetontology.net/realmLandGlacial/Till> a owl:Class .

<http://sweetontology.net/realmLandGlacial/Thermokarst> a owl:Class ;
	rdfs:subClassOf <http://sweetontology.net/realmLandGlacial/GlacialLandform> ;
	rdfs:comment "A land surface characterised by very irregular surfaces of marshy hollows and small hummocks formed as ice-rich permafrost thaws."@en .

<http://sweetontology.net/realmLandGlacial/UShapedValley> a owl:Class ;
	rdfs:subClassOf <http://sweetontology.net/realmLandGlacial/GlacialLandform> .
