@prefix planet: <http://sweetontology.net/realm/> .
@prefix climate: <http://sweetontology.net/phenPlanetClimate/> .
@prefix time: <http://sweetontology.net/reprTimeSeason/> .
@prefix ptime: <http://sweetontology.net/propTime/> .
@prefix math: <http://sweetontology.net/reprMath/> .
@prefix temp: <http://sweetontology.net/propTemperature/> .
@prefix thic: <http://sweetontology.net/propSpaceThickness/> .
@prefix cate: <http://sweetontology.net/propCategorical/> .
@prefix rela: <http://sweetontology.net/rela/> .
@prefix crela: <http://sweetontology.net/relaClimate/> .
@prefix mrela: <http://sweetontology.net/relaMath/> .
@prefix srela: <http://sweetontology.net/relaSci/> .
@prefix sreg: <http://sweetontology.net/realmRegion/> .
@prefix zone: <http://sweetontology.net/realmClimateZone/> .
@prefix owl: <http://www.w3.org/2002/07/owl#> .
@prefix rdf: <http://www.w3.org/1999/02/22-rdf-syntax-ns#> .
@prefix rdfs: <http://www.w3.org/2000/01/rdf-schema#> .
@prefix xsd: <http://www.w3.org/2001/XMLSchema#> .

<http://sweetontology.net/realmClimateZone> a owl:Ontology ;
	owl:versionInfo "3.0.0" ;
	rdfs:label "SWEET Ontology" ;
	owl:imports <http://sweetontology.net/reprTimeSeason> , <http://sweetontology.net/propTime> , <http://sweetontology.net/reprMath> , <http://sweetontology.net/propTemperature> , <http://sweetontology.net/realmRegion> , <http://sweetontology.net/realm> , <http://sweetontology.net/rela> , <http://sweetontology.net/relaClimate> , <http://sweetontology.net/relaMath> , <http://sweetontology.net/relaSci> , <http://sweetontology.net/propCategorical> , <http://sweetontology.net/phenPlanetClimate> .

owl:versionInfo a owl:AnnotationProperty .

zone:ClimateClassification a owl:Class ;
	rdfs:subClassOf cate:Category .

zone:ClimateZoneType a owl:Class ;
	rdfs:subClassOf zone:ClimateClassification .

zone:MarineClimate a owl:Class ;
	rdfs:subClassOf zone:ClimateClassification , _:node1boameed5x1 .

_:node1boameed5x1 a owl:Restriction ;
	owl:onProperty rela:hasRealm ;
	owl:someValuesFrom planet:Ocean .

zone:MarineClimate rdfs:comment "(Also called maritime climate, oceanic climate.) A regional climate under the predominant influence of the sea, characterized by relatively small seasonal variations and high atmospheric moisture content; the antithesis of a continental climate."@en .

zone:RainShadow a owl:Class ;
	rdfs:subClassOf zone:ClimateZoneType ;
	rdfs:comment "A region of sharply reduced precipitation on the lee side of an orographic barrier, as compared with regions upwind of the barrier."@en .

zone:Doldrums a owl:Class ;
	rdfs:subClassOf zone:ClimateZoneType , _:node1boameed5x2 .

_:node1boameed5x2 a owl:Restriction ;
	owl:onProperty rela:hasRealm ;
	owl:hasValue sreg:LowLatitude .

zone:Doldrums rdfs:comment "A nautical term for the equatorial trough, with special reference to the light and variable nature of the winds."@en .

zone:DesertClimateZone a owl:Class ;
	rdfs:subClassOf zone:ClimateZoneType .

zone:IntertropicalConvergenceZone a owl:Class ;
	rdfs:subClassOf zone:ClimateZoneType ;
	owl:equivalentClass zone:ITCZ ;
	rdfs:subClassOf _:node1boameed5x3 .

_:node1boameed5x3 a owl:Restriction ;
	owl:onProperty rela:hasRealm ;
	owl:allValuesFrom zone:Equator .

zone:ITCZ a owl:Class .

zone:SubtropicalClimateZone a owl:Class ;
	rdfs:subClassOf zone:ClimateZoneType .

zone:TropicalClimateZone a owl:Class ;
	rdfs:subClassOf zone:ClimateZoneType .

zone:DryWinterClimate a owl:Class ;
	rdfs:subClassOf zone:ClimateClassification , _:node1boameed5x4 .

_:node1boameed5x4 a owl:Restriction ;
	owl:onProperty crela:hasDrySeason ;
	owl:hasValue time:Winter .

zone:WetSummerClimate a owl:Class ;
	rdfs:subClassOf zone:ClimateClassification , _:node1boameed5x5 .

_:node1boameed5x5 a owl:Restriction ;
	owl:onProperty crela:hasWetSeason ;
	owl:hasValue time:Summer .

zone:WetSummerDryWinterClimate a owl:Class ;
	rdfs:subClassOf zone:DryWinterClimate , zone:WetSummerClimate .

zone:A a owl:Class ;
	owl:equivalentClass zone:TropicalClimate ;
	rdfs:subClassOf zone:ClimateClassification ;
	rdfs:comment "The A climate classification, also known as the Tropical climate classification, is characterized as being consistently warm with all months averaging above 18 degrees C and having annual precipitation exceeds potential evapotranspiration (POTET)."@en ;
	rdfs:subClassOf _:node1boameed5x6 .

_:node1boameed5x6 a owl:Restriction ;
	owl:onProperty crela:hasAverageAnnualPrecipitation ;
	owl:hasValue _:node1boameed5x7 .

_:node1boameed5x7 a thic:PrecipitationRange ;
	srela:hasLowerQuantity thic:AnnualPotentialEvapotranspiration .

zone:A rdfs:subClassOf _:node1boameed5x8 .

_:node1boameed5x8 a owl:Restriction ;
	owl:onProperty crela:hasAverageMonthlyTemperature ;
	owl:hasValue _:node1boameed5x9 .

_:node1boameed5x9 a temp:TemperatureRange ;
	mrela:hasLowerBound "18"^^xsd:integer .

zone:TropicalClimate a owl:Class .

zone:B a owl:Class ;
	owl:equivalentClass zone:DryClimate ;
	rdfs:subClassOf zone:ClimateClassification ;
	rdfs:comment "Potential evapotranspiration (POTET) exceeds precipitation in all B climates. Subdivisions are based on precipitation timing and amount and mean annual temperature."@en ;
	rdfs:subClassOf _:node1boameed5x10 .

_:node1boameed5x10 a owl:Restriction ;
	owl:onProperty crela:hasAverageAnnualPrecipitation ;
	owl:hasValue _:node1boameed5x11 .

_:node1boameed5x11 a thic:PrecipitationRange ;
	srela:hasLowerQuantity thic:AnnualPotentialEvapotranspiration .

zone:DryClimate a owl:Class .

zone:C a owl:Class ;
	rdfs:subClassOf zone:ClimateClassification ;
	owl:equivalentClass zone:TemperateClimate ;
	rdfs:subClassOf _:node1boameed5x12 .

_:node1boameed5x12 a owl:Restriction ;
	owl:onProperty crela:hasAverageColdestMonthTemperature ;
	owl:hasValue _:node1boameed5x13 .

_:node1boameed5x13 a temp:TemperatureRange ;
	mrela:hasLowerBound "0"^^xsd:integer ;
	mrela:hasUpperBound "18"^^xsd:integer .

zone:C rdfs:subClassOf _:node1boameed5x14 .

_:node1boameed5x14 a owl:Restriction ;
	owl:onProperty crela:hasAverageWarmestMonthTemperature ;
	owl:hasValue _:node1boameed5x15 .

_:node1boameed5x15 a temp:TemperatureRange ;
	mrela:hasLowerBound "10"^^xsd:integer ;
	mrela:hasUpperBound "22"^^xsd:integer .

zone:TemperateClimate a owl:Class .

zone:D a owl:Class ;
	rdfs:subClassOf zone:ClimateClassification , _:node1boameed5x16 .

_:node1boameed5x16 a owl:Restriction ;
	owl:onProperty crela:hasAverageColdestMonthTemperature ;
	owl:hasValue _:node1boameed5x17 .

_:node1boameed5x17 a temp:TemperatureRange ;
	mrela:hasUpperBound "0"^^xsd:integer .

zone:D rdfs:subClassOf _:node1boameed5x18 .

_:node1boameed5x18 a owl:Restriction ;
	owl:onProperty crela:hasAverageWarmestMonthTemperature ;
	owl:hasValue _:node1boameed5x19 .

_:node1boameed5x19 a temp:TemperatureRange ;
	mrela:hasLowerBound "10"^^xsd:integer .

zone:D rdfs:comment "The D climate classification, also known as the microthermal climate classification,  is characterized by by having the warmest month of the year above 10 degree C and the coldest below 0 degree C."@en .

zone:E a owl:Class ;
	rdfs:subClassOf zone:ClimateClassification .

zone:Af a zone:A ;
	owl:sameAs zone:TropicalRainForestClimate ;
	crela:hasAverageMonthlyPrecipitation _:node1boameed5x20 .

_:node1boameed5x20 a thic:PrecipitationRange_cm ;
	mrela:hasLowerBound "6"^^xsd:integer .

zone:Af rdfs:comment "The Af climate classification, also known as the tropical rain forest climate classification, is characterized by monthly precipitation in excess of 6 cm all months out of year."@en .

zone:TropicalRainForestClimate a zone:A .

zone:Am a zone:A ;
	owl:sameAs zone:TropicalMonsoonClimate ;
	crela:hasAverageDrySeasonPrecipitation _:node1boameed5x21 .

_:node1boameed5x21 a thic:PrecipitationRange_cm ;
	mrela:hasUpperBound "6"^^xsd:integer .

zone:Am crela:hasAverageITCZDominanceDuration _:node1boameed5x22 .

_:node1boameed5x22 a ptime:MonthRange ;
	mrela:hasLowerBound "6"^^xsd:integer .

zone:Am rdfs:comment "The Am climate classification, also known as Tropical Monsoon Climate, is characterized by a short marked dry season with 1 or more months receiving less than 6 cm of precipitation, an otherwise excessively wet rainy season, and ITCZ dominance for 6 - 12 months out of the year."@en .

zone:TropicalMonsoonClimate a zone:A .

zone:Aw a zone:A ;
	owl:sameAs zone:TropicalSavannaClimate ;
	a zone:WetSummerDryWinterClimate ;
	crela:hasAverageITCZDominanceDuration _:node1boameed5x23 .

_:node1boameed5x23 a ptime:MonthRange ;
	mrela:hasUpperBound "6"^^xsd:integer .

zone:Aw rdfs:comment "The Aw climate classification, also known as Tropical Savanna climate classification, is characterized by a summer wet season, winter dry season, and ITCZ dominance for 6 months or less."@en .

zone:TropicalSavannaClimate a zone:A .

zone:BS a zone:B ;
	owl:sameAs zone:SemiAridClimate ;
	crela:hasAverageAnnualPrecipitation _:node1boameed5x24 .

_:node1boameed5x24 a thic:PrecipitationRange ;
	srela:hasLowerQuantity thic:AnnualHalfPotentialEvapotranspiration ;
	srela:hasUpperQuantity thic:AnnualPotentialEvapotranspiration .

zone:BS rdfs:comment "The BS climate classification, also known as semiarid climate classification, is characterized by having precipitation amounts greater than 1/2 potential evapotranspiration (POTET), but not equal to it."@en .

zone:SemiAridClimate a zone:B .

zone:BSh a zone:B ;
	owl:sameAs zone:HotLowLatitudeSteppeClimate ;
	rdfs:comment "The BSh climate classification, also known as the hot low-latitude steppe, is characterized by having mean annual temperatures greater than 18 degree C."@en ;
	crela:hasAverageAnnualTemperature _:node1boameed5x25 .

_:node1boameed5x25 a temp:TemperatureRange ;
	mrela:hasLowerBound "18"^^xsd:integer .

zone:HotLowLatitudeSteppeClimate a zone:B .

zone:BSk a zone:B ;
	owl:sameAs zone:ColdMidlatitudeSteppeClimate ;
	crela:hasAverageAnnualTemperature _:node1boameed5x26 .

_:node1boameed5x26 a temp:TemperatureRange ;
	mrela:hasUpperBound "18"^^xsd:integer .

zone:BSk rdfs:comment "The BSk climate classification, also known as cold midlatitude steppe climate classification, is characterized by having mean annual temperatures less than 18 degree C."@en .

zone:ColdMidlatitudeSteppeClimate a zone:B .

zone:BW a zone:B ;
	owl:sameAs zone:AridClimate , zone:Arid ;
	rdfs:comment "The BW climate classification, also known as the arid climate classification, is characterized by having precipitation amounts less than 1/2 potential evapotranspiration (POTET)."@en ;
	crela:hasAverageAnnualPrecipitation _:node1boameed5x27 .

_:node1boameed5x27 a thic:PrecipitationRange ;
	srela:hasUpperQuantity thic:AnnualHalfPotentialEvapotranspiration .

zone:AridClimate a zone:B .

zone:Arid a zone:B .

zone:BWh a zone:B ;
	owl:sameAs zone:HotLowLatitudeDesertClimate ;
	rdfs:comment "the BWh climate classification, also known as the hot low-latitude desert, is characterized by having mean annual temperatures greater than 18 degree C."@en ;
	crela:hasAverageAnnualTemperature _:node1boameed5x28 .

_:node1boameed5x28 a temp:TemperatureRange ;
	mrela:hasLowerBound "18"^^xsd:integer .

zone:HotLowLatitudeDesertClimate a zone:B .

zone:BWk a zone:B ;
	owl:sameAs zone:ColdMidlatitudeDesertClimate ;
	rdfs:comment "The BWk climate classification, also known as the cold midlatitude desert, is characterized by having mean annual temperatures less than 18 degree C."@en ;
	crela:hasAverageAnnualTemperature _:node1boameed5x29 .

_:node1boameed5x29 a temp:TemperatureRange ;
	mrela:hasUpperBound "18"^^xsd:integer .

zone:ColdMidlatitudeDesertClimate a zone:B .

zone:Cfa a zone:C ;
	crela:hasAverageWarmestMonthTemperature _:node1boameed5x30 .

_:node1boameed5x30 a temp:TemperatureRange ;
	mrela:hasLowerBound "22"^^xsd:integer .

zone:Cfa rdfs:comment "The Cfa climate classification is characterized by year-round precipitation, hot summers, and having the warmest month above 22 degree C."@en .

zone:Cfb a zone:C ;
	crela:hasAverageWarmestMonthTemperature _:node1boameed5x31 .

_:node1boameed5x31 a temp:TemperatureRange ;
	mrela:hasUpperBound "22"^^xsd:integer .

zone:Cfb crela:hasAverageWinterDuration _:node1boameed5x32 .

_:node1boameed5x32 a ptime:MonthRange ;
	mrela:hasLowerBound "4"^^xsd:integer .

zone:Cfb rdfs:comment "The Cfb climate classfication receives year-round precipitation, its warmest month is below 22 degree C and has 4 months above 10 degree C."@en .

zone:Cfc a zone:C ;
	crela:hasAverageWinterDuration _:node1boameed5x33 .

_:node1boameed5x33 a ptime:MonthRange ;
	mrela:hasLowerBound "1"^^xsd:integer ;
	mrela:hasUpperBound "3"^^xsd:integer .

zone:Cfc rdfs:comment "The Cfc climate classification is charactericized by year-round precipitation and having 1 - 3 months with temperatures above 10 degree C."@en .

zone:Csa a zone:C ;
	crela:hasWetSeason time:Winter ;
	crela:hasDrySeason time:Summer ;
	crela:hasAverageWarmestMonthTemperature _:node1boameed5x34 .

_:node1boameed5x34 a temp:TemperatureRange ;
	mrela:hasLowerBound "22"^^xsd:integer .

zone:Csa rdfs:comment "The Csa climate classification is characterized by pronounced summer droughts with 70% of precipitation in the winter and hot summers with its warmest month above 22 degree C."@en .

zone:Csb a zone:C , zone:WetSummerDryWinterClimate ;
	crela:hasAverageWarmestMonthTemperature _:node1boameed5x35 .

_:node1boameed5x35 a temp:TemperatureRange ;
	mrela:hasLowerBound "10"^^xsd:integer ;
	mrela:hasUpperBound "22"^^xsd:integer .

zone:Cwa a zone:C , zone:WetSummerDryWinterClimate ;
	crela:hasAverageWarmestMonthTemperature _:node1boameed5x36 .

_:node1boameed5x36 a temp:TemperatureRange ;
	mrela:hasLowerBound "22"^^xsd:integer .

zone:Cwa rdfs:comment "the Cwa climate classification is characterized by winter drought, summer's wettest month getting 10 times more precipitation than driest winter month, and the warmest month being above 22 degree C."@en .

zone:Dfa a zone:D ;
	crela:hasAverageWarmestMonthTemperature _:node1boameed5x37 .

_:node1boameed5x37 a temp:TemperatureRange ;
	mrela:hasLowerBound "22"^^xsd:integer .

zone:Dfa rdfs:comment "The Dfa climate classification is characterized by having year-round precipitation and warmest month temperatures above 22 degree C."@en .

zone:Dfb a zone:D ;
	rdfs:comment "The Dfb climate classifcation is characterized by having year-round precipitation and warmest month temperatures below 22 degree C."@en ;
	crela:hasAverageWarmestMonthTemperature _:node1boameed5x38 .

_:node1boameed5x38 a temp:TemperatureRange ;
	mrela:hasUpperBound "22"^^xsd:integer .

zone:Dfc a zone:D ;
	crela:hasAverageWinterDuration _:node1boameed5x39 .

_:node1boameed5x39 a ptime:MonthRange ;
	mrela:hasLowerBound "1"^^xsd:integer ;
	mrela:hasUpperBound "4"^^xsd:integer .

zone:Dfc rdfs:comment "The Dfc climate classification is characterized by having year-round precipitation and having 1 - 4 months above 10 degree C."@en .

zone:Dwa a zone:D , zone:DryWinterClimate ;
	crela:hasAverageWarmestMonthTemperature _:node1boameed5x40 .

_:node1boameed5x40 a temp:TemperatureRange ;
	mrela:hasLowerBound "22"^^xsd:integer .

zone:Dwa rdfs:comment "The Dwa climate classification is characterized by winter drought and warmest month temperatures above 22 degree C."@en .

zone:Dwb a zone:D , zone:DryWinterClimate ;
	crela:hasAverageWarmestMonthTemperature _:node1boameed5x41 .

_:node1boameed5x41 a temp:TemperatureRange ;
	mrela:hasUpperBound "22"^^xsd:integer .

zone:Dwb rdfs:comment "The Dwb climate classification is characterized by winter drought and warmest month temperatures below 22 degree C."@en .

zone:Dwc a zone:D , zone:DryWinterClimate ;
	rdfs:comment "The Dwc climate classification is characterized by winter drought and haviong 1 - 4 months with temperatures above 10 degrees C."@en ;
	crela:hasAverageWinterDuration _:node1boameed5x42 .

_:node1boameed5x42 a ptime:MonthRange ;
	mrela:hasLowerBound "1"^^xsd:integer ;
	mrela:hasUpperBound "4"^^xsd:integer .

zone:Dwd a zone:D , zone:DryWinterClimate ;
	rdfs:comment "The Dwd climate classification is characterized by winter drought and having coldest month temperatures below -38 degree C (in Siberia only)."@en ;
	crela:hasAverageColdestMonthTemperature _:node1boameed5x43 .

_:node1boameed5x43 a temp:TemperatureRange ;
	mrela:hasUpperBound "-38"^^xsd:integer .

zone:EF a zone:E ;
	owl:sameAs zone:IceCapClimate ;
	rdfs:comment "The EF climate classification, also known as the Ice Cap climate classification, is characterized by having warmest month temperatures below 0 degrees C and having precipitation exceeding very small potential evapotranspiration (POTET)."@en ;
	crela:hasAverageWarmestMonthTemperature _:node1boameed5x44 .

_:node1boameed5x44 a temp:TemperatureRange ;
	mrela:hasUpperBound "0"^^xsd:integer .

zone:EF crela:hasAverageAnnualPrecipitation _:node1boameed5x45 .

_:node1boameed5x45 a thic:PrecipitationRange ;
	srela:hasLowerQuantity thic:AnnualPotentialEvapotranspiration .

zone:IceCapClimate a zone:E .

zone:EM a zone:E ;
	owl:sameAs zone:PolarMarineClimate ;
	rdfs:comment "The EM climate classification, also known as the polar marine climate classification, is characterized by all months having temperatures above -7 degree C, warmest month above 0 degree C, and annual temperatures less than 17 degree C."@en ;
	crela:hasAverageMonthlyTemperature _:node1boameed5x46 .

_:node1boameed5x46 a temp:TemperatureRange ;
	mrela:hasLowerBound "-7"^^xsd:integer .

zone:EM crela:hasAverageWarmestMonthTemperature _:node1boameed5x47 .

_:node1boameed5x47 a temp:TemperatureRange ;
	mrela:hasLowerBound "0"^^xsd:integer .

zone:EM crela:hasAverageAnnualTemperature _:node1boameed5x48 .

_:node1boameed5x48 a temp:TemperatureRange ;
	mrela:hasUpperBound "17"^^xsd:integer .

zone:PolarMarineClimate a zone:E .

zone:ET a zone:E ;
	owl:sameAs zone:TundraClimate ;
	crela:hasAverageSnowCoverDuration _:node1boameed5x49 .

_:node1boameed5x49 a ptime:MonthRange ;
	mrela:hasLowerBound "8"^^xsd:integer ;
	mrela:hasUpperBound "10"^^xsd:integer .

zone:ET crela:hasWarmestMonthTemperature _:node1boameed5x50 .

_:node1boameed5x50 a temp:TemperatureRange ;
	mrela:hasLowerBound "0"^^xsd:integer ;
	mrela:hasUpperBound "10"^^xsd:integer .

zone:ET crela:hasAverageAnnualPrecipitation _:node1boameed5x51 .

_:node1boameed5x51 a thic:PrecipitationRange ;
	srela:hasLowerQuantity thic:AnnualPotentialEvapotranspiration .

zone:ET rdfs:comment "The ET climate classification, also known as the tundra climate classification, is characterizex by warmest month temperatures between 0 - 10 degree C, precipitation exceeds small potential evapotranspiration demand, and has snow cover 8 - 10 months out of the year."@en .

zone:TundraClimate a zone:E .

zone:Equator a owl:Class ;
	rdfs:subClassOf zone:TropicalClimateZone .
