@prefix time: <http://sweetontology.net/propTime/> .
@prefix stime: <http://sweetontology.net/stateTime/> .
@prefix units: <http://sweetontology.net/reprSciUnits/> .
@prefix ordi: <http://sweetontology.net/propOrdinal/> .
@prefix mtime: <http://sweetontology.net/reprTime/> .
@prefix screla: <http://sweetontology.net/relaSci/> .
@prefix trela: <http://sweetontology.net/relaTime/> .
@prefix owl: <http://www.w3.org/2002/07/owl#> .
@prefix xsd: <http://www.w3.org/2001/XMLSchema#> .
@prefix rdf: <http://www.w3.org/1999/02/22-rdf-syntax-ns#> .
@prefix rdfs: <http://www.w3.org/2000/01/rdf-schema#> .

<http://sweetontology.net/stateTime> a owl:Ontology ;
	owl:versionInfo "3.0.0" ;
	rdfs:label "SWEET Ontology" ;
	owl:imports <http://sweetontology.net/propTime> , <http://sweetontology.net/reprSciUnits> , <http://sweetontology.net/relaTime> , <http://sweetontology.net/relaSci> , <http://sweetontology.net/reprTime> , <http://sweetontology.net/propOrdinal> .

<http://sweetontology.net/stateTime/1hour> a time:Duration ;
	screla:hasNumericValue "1"^^xsd:double ;
	screla:hasUnit units:hour .

<http://sweetontology.net/stateTime/12hour> a time:Duration ;
	screla:hasNumericValue "12"^^xsd:double ;
	screla:hasUnit units:hour .

<http://sweetontology.net/stateTime/1day> a time:Duration ;
	screla:hasNumericValue "1"^^xsd:double ;
	screla:hasUnit units:day .

<http://sweetontology.net/stateTime/5day> a time:Duration ;
	screla:hasNumericValue "5"^^xsd:double ;
	screla:hasUnit units:day .

<http://sweetontology.net/stateTime/1week> a time:Duration ;
	screla:hasNumericValue "1"^^xsd:double ;
	screla:hasUnit units:week .

<http://sweetontology.net/stateTime/2week> a time:Duration ;
	screla:hasNumericValue "2"^^xsd:double ;
	screla:hasUnit units:week .

<http://sweetontology.net/stateTime/1month> a time:Duration ;
	screla:hasNumericValue "1"^^xsd:double ;
	screla:hasUnit units:month .

<http://sweetontology.net/stateTime/3month> a time:Duration ;
	screla:hasNumericValue "3"^^xsd:double ;
	screla:hasUnit units:month .

<http://sweetontology.net/stateTime/6month> a time:Duration ;
	screla:hasNumericValue "6"^^xsd:double ;
	screla:hasUnit units:month .

<http://sweetontology.net/stateTime/1year> a time:Duration ;
	screla:hasNumericValue "1"^^xsd:double ;
	screla:hasUnit units:year .

<http://sweetontology.net/stateTime/2year> a time:Duration ;
	screla:hasNumericValue "2"^^xsd:double ;
	screla:hasUnit units:year .

<http://sweetontology.net/stateTime/10year> a time:Duration ;
	screla:hasNumericValue "10"^^xsd:double ;
	screla:hasUnit units:year .

stime:ShortLived a time:Duration .

stime:Age a owl:Class ;
	rdfs:subClassOf stime:GeologicTimeUnit , _:node1boamerp7x1 .

_:node1boamerp7x1 a owl:Restriction ;
	owl:onProperty trela:temporalPartOf ;
	owl:someValuesFrom stime:Epoch .

stime:Age rdfs:comment "Epochs are divided into ages [millions of years] [Wikipedia]"@en .

stime:Epoch a owl:Class ;
	rdfs:subClassOf stime:GeologicTimeUnit , _:node1boamerp7x2 .

_:node1boamerp7x2 a owl:Restriction ;
	owl:onProperty trela:temporalPartOf ;
	owl:someValuesFrom stime:Period .

stime:Epoch rdfs:comment "Periods are divided into epochs [tens of millions of years] [Wikipedia]"@en .

stime:Period a owl:Class ;
	rdfs:subClassOf stime:GeologicTimeUnit , _:node1boamerp7x3 .

_:node1boamerp7x3 a owl:Restriction ;
	owl:onProperty trela:temporalPartOf ;
	owl:someValuesFrom stime:Era .

stime:Period rdfs:comment "Eras are divided into periods. [Wikipedia]"@en .

stime:Era a owl:Class ;
	rdfs:subClassOf stime:GeologicTimeUnit , _:node1boamerp7x4 .

_:node1boamerp7x4 a owl:Restriction ;
	owl:onProperty trela:temporalPartOf ;
	owl:someValuesFrom stime:Eon .

stime:Era rdfs:comment "Eons are divided into eras [several hundred million years] [Wikipedia]"@en .

stime:Eon a owl:Class ;
	rdfs:subClassOf stime:GeologicTimeUnit , _:node1boamerp7x5 .

_:node1boamerp7x5 a owl:Restriction ;
	owl:onProperty trela:temporalPartOf ;
	owl:someValuesFrom stime:Supereon .

stime:Eon rdfs:comment "Supereons are divided into eons.  [billions of years] [Wikipedia]"@en .

stime:Supereon a owl:Class ;
	rdfs:subClassOf stime:GeologicTimeUnit ;
	rdfs:comment "The largest defined unit of time is the supereon, composed of eons.] [Wikipedia]"@en .

stime:GeologicTimeUnit a owl:Class ;
	rdfs:subClassOf time:Duration ;
	rdfs:comment "The subdivisions of geologic time. The table of geologic time spans are dates and nomenclature defined by the International Commission on Stratigraphy. [Wikipedia]"@en .

stime:NeotectonicPeriod a owl:Class ;
	rdfs:subClassOf mtime:TimeReference .

stime:Ancient a ordi:Age ;
	trela:olderThan stime:New .

stime:Antiquated a ordi:Age ;
	trela:olderThan stime:New .

stime:Antique a ordi:Age ;
	trela:olderThan stime:New .

stime:Fresh a ordi:Age .

stime:Incipient a ordi:Age .

stime:Lifetime a ordi:Age .

stime:New a ordi:Age .

stime:Young a ordi:Age .

stime:Old a ordi:Age ;
	trela:olderThan stime:Young , stime:New .

stime:Past a ordi:Age ;
	trela:olderThan stime:Present .

stime:Present a ordi:Age ;
	trela:olderThan stime:Future .

stime:Future a ordi:Age .

stime:Prehistoric a ordi:Age .

stime:Primordial a ordi:Age .

stime:Recent a ordi:Age .

stime:Immature a ordi:Age .

stime:Mature a ordi:Age ;
	trela:olderThan stime:Immature .

stime:Young a ordi:Age .
